Add files via upload

Binary_operations.thy
@@ -1,5 +1,5 @@
 theory Binary_operations
- imports Bij_betw_simplicial_complex_bool_func
+  imports Bij_betw_simplicial_complex_bool_func
 begin
 
 definition bool_fun_or :: "(bool^'n \<Rightarrow> bool) \<Rightarrow> (bool^'n \<Rightarrow> bool) \<Rightarrow> (bool^'n \<Rightarrow> bool)"
@@ -8,11 +8,68 @@ definition bool_fun_or :: "(bool^'n \<Rightarrow> bool) \<Rightarrow> (bool^'n \
 definition bool_fun_and :: "(bool^'n \<Rightarrow> bool) \<Rightarrow> (bool^'n \<Rightarrow> bool) \<Rightarrow> (bool^'n \<Rightarrow> bool)"
   where "(bool_fun_and f g) x \<equiv> (f x) \<and> (g x)"
 
-definition bool_fun_ast :: "(bool^'n \<Rightarrow> bool) \<Rightarrow> (bool^'m \<Rightarrow> bool) \<Rightarrow> (bool^'n \<Rightarrow> bool^'m \<Rightarrow> bool)"
+definition bool_fun_ast :: "(bool^'n \<Rightarrow> bool) \<Rightarrow> (bool^'m \<Rightarrow> bool) \<Rightarrow> ((bool^'n) \<Rightarrow>(bool^'m) \<Rightarrow> bool)"
   where "(bool_fun_ast f g) x y \<equiv> (f x) \<and> (g y)"
 
-definition set_ast :: "('a set) \<Rightarrow> ('a set) \<Rightarrow> ('a set)"
-  where "set_ast A B = {}"
+definition
+  simplicial_complex_induced_by_monotone_boolean_function_ast 
+    :: "(bool^'n::class_mod_type => bool^'m::class_mod_type \<Rightarrow> bool) => ('n set * 'm set) set"
+  where "simplicial_complex_induced_by_monotone_boolean_function_ast f = 
+        {z. \<exists>x y. f x y \<and> ((ceros_of_boolean_input x), (ceros_of_boolean_input y)) = z}"
+
+lemma fst_es_simplice:
+  "a \<in> simplicial_complex_induced_by_monotone_boolean_function_ast f 
+\<Longrightarrow> (\<exists>x y. f x y \<and> (ceros_of_boolean_input x) = fst(a))"
+  by (smt (verit) fst_conv mem_Collect_eq simplicial_complex_induced_by_monotone_boolean_function_ast_def)
+
+lemma snd_es_simplice:
+  "a \<in> simplicial_complex_induced_by_monotone_boolean_function_ast f 
+\<Longrightarrow> (\<exists>x y. f x y \<and> (ceros_of_boolean_input y) = snd(a))"
+  by (smt (verit) snd_conv mem_Collect_eq simplicial_complex_induced_by_monotone_boolean_function_ast_def)
+
+definition set_ast :: "('a set) \<Rightarrow> ('b set) \<Rightarrow> (('a*'b) set)"
+  where "set_ast A B \<equiv> {c. \<exists>a\<in>A. \<exists>b\<in>B. c = (a,b)}"
+
+definition set_fst :: "('a::class_mod_type*'b::class_mod_type) set \<Rightarrow> 'a set"
+  where "set_fst AB = {a. \<exists>ab\<in>AB. a = fst ab}"
+
+value "set_fst {a, b}"
+
+lemma set_fst_simp [simp]: "set_fst (x \<times> y) = x"
+proof
+  show "set_fst (x \<times> y) \<subseteq> x"
+    by (smt (verit) SigmaE mem_Collect_eq prod.sel(1) set_fst_def subsetI)
+  show "x \<subseteq> set_fst (x \<times> y)"
+  proof
+    fix a::"'a"
+    assume "a \<in> x"
+    then have "\<exists>b\<in>y. (a,b)\<in>(x\<times>y)"
+      by auto
+    thus "a \<in> set_fst (x \<times> y)"
+      by auto
+  qed
+qed
+
+definition set_snd :: "('a*'b) set \<Rightarrow> 'b set"
+  where "set_snd AB = {b. \<exists>ab\<in>AB. b = snd(ab)}"
+
+definition bool_fun_times :: "(bool^('n::class_mod_type) \<Rightarrow> bool) \<Rightarrow> (bool^('m::class_mod_type) \<Rightarrow> bool) \<Rightarrow> (bool^('n*'m) \<Rightarrow> bool)"
+  where "(bool_fun_times f g) x \<equiv>
+     f (bool_vec_from_simplice (set_fst (ceros_of_boolean_input x)))
+   \<and> g (bool_vec_from_simplice (set_snd (ceros_of_boolean_input x)))"
+
+(* La siguiente condición causa que el teorema pertinente sea incorrecto:
+ \<and> (\<nexists>c. \<exists>d\<in>(ceros_of_boolean_input x). c\<in>(ceros_of_boolean_input x) \<and> (fst c < fst d) \<and> (snd c > snd d))*)
+
+definition
+  simplicial_complex_induced_by_monotone_boolean_function_times 
+    :: "(bool^('n::class_mod_type*'m::class_mod_type) \<Rightarrow> bool) => (('n set)*('m set)) set"
+  where "simplicial_complex_induced_by_monotone_boolean_function_times f = 
+        {z. \<exists>x y. f (bool_vec_from_simplice (x \<times> y)) \<and> (x, y) = z}"
+
+lemma simp_ceros [simp]: "ceros_of_boolean_input (bool_vec_from_simplice (x \<times> y)) = x \<times> y"
+  unfolding bool_vec_from_simplice_def
+  unfolding ceros_of_boolean_input_def by auto
 
 lemma eq_union_or: 
 "simplicial_complex_induced_by_monotone_boolean_function (bool_fun_or f g)
@@ -83,6 +140,88 @@ next
       by (smt (z3) sigma bool_fun_and_def mem_Collect_eq simplicial_complex_induced_by_monotone_boolean_function_def)
     thus "\<sigma> \<in> simplicial_complex_induced_by_monotone_boolean_function f \<inter> simplicial_complex_induced_by_monotone_boolean_function g"
       by auto
+  qed
+qed
+
+lemma eq_ast: 
+"simplicial_complex_induced_by_monotone_boolean_function_ast (bool_fun_ast f g)
+= set_ast (simplicial_complex_induced_by_monotone_boolean_function f) (simplicial_complex_induced_by_monotone_boolean_function g)"
+proof
+  show "set_ast (simplicial_complex_induced_by_monotone_boolean_function f) (simplicial_complex_induced_by_monotone_boolean_function g) \<subseteq> simplicial_complex_induced_by_monotone_boolean_function_ast (bool_fun_ast f g)"
+  proof
+    fix \<gamma>::"'a set*'b set"
+    assume pert: "\<gamma> \<in> set_ast (simplicial_complex_induced_by_monotone_boolean_function f) (simplicial_complex_induced_by_monotone_boolean_function g)"
+    hence "(fst \<gamma>) \<in> simplicial_complex_induced_by_monotone_boolean_function f"
+      unfolding set_ast_def
+      by auto
+    hence sigma: "f (bool_vec_from_simplice (fst \<gamma>))"
+      by (metis (mono_tags, lifting) bool_vec_set_from_simplice_set_def boolean_function_from_simplicial_complex_def boolean_function_from_simplicial_complex_simplicial_complex_induced_by_monotone_boolean_function_id mem_Collect_eq)
+    from pert have "(snd \<gamma>) \<in> simplicial_complex_induced_by_monotone_boolean_function g"
+      unfolding set_ast_def
+      by auto
+    hence tau: "g (bool_vec_from_simplice (snd \<gamma>))"
+      by (metis (mono_tags, lifting) bool_vec_set_from_simplice_set_def boolean_function_from_simplicial_complex_def boolean_function_from_simplicial_complex_simplicial_complex_induced_by_monotone_boolean_function_id mem_Collect_eq)
+    from sigma and tau have sigtau: "bool_fun_ast f g (bool_vec_from_simplice (fst \<gamma>)) (bool_vec_from_simplice (snd \<gamma>))"
+      unfolding bool_fun_ast_def
+      by auto
+    from sigtau show "\<gamma> \<in> simplicial_complex_induced_by_monotone_boolean_function_ast (bool_fun_ast f g)"
+      using bool_vec_from_simplice_def ceros_of_boolean_input_in_set mem_Collect_eq simplicial_complex_induced_by_monotone_boolean_function_ast_def
+      by fastforce
+  qed
+next
+  show "simplicial_complex_induced_by_monotone_boolean_function_ast (bool_fun_ast f g) \<subseteq> set_ast (simplicial_complex_induced_by_monotone_boolean_function f) (simplicial_complex_induced_by_monotone_boolean_function g)"
+  proof
+    fix \<gamma>::"'a set*'b set"
+    assume pert: "\<gamma> \<in> simplicial_complex_induced_by_monotone_boolean_function_ast (bool_fun_ast f g)"
+    hence sigma: "(fst \<gamma>) \<in> simplicial_complex_induced_by_monotone_boolean_function f"
+      by (smt (verit) bool_fun_ast_def fst_es_simplice mem_Collect_eq simplicial_complex_induced_by_monotone_boolean_function_def)
+    from pert have tau: "(snd \<gamma>) \<in> simplicial_complex_induced_by_monotone_boolean_function g"
+      by (smt (verit) bool_fun_ast_def snd_es_simplice mem_Collect_eq simplicial_complex_induced_by_monotone_boolean_function_def)
+    from sigma and tau show "\<gamma> \<in> set_ast (simplicial_complex_induced_by_monotone_boolean_function f) (simplicial_complex_induced_by_monotone_boolean_function g)"
+      using set_ast_def
+      by force
+  qed
+qed
+
+
+lemma eq_times: 
+"simplicial_complex_induced_by_monotone_boolean_function_times (bool_fun_times f g)
+= (simplicial_complex_induced_by_monotone_boolean_function f) \<times> (simplicial_complex_induced_by_monotone_boolean_function g)"
+proof
+  show "(simplicial_complex_induced_by_monotone_boolean_function f) \<times> (simplicial_complex_induced_by_monotone_boolean_function g) \<subseteq> simplicial_complex_induced_by_monotone_boolean_function_times (bool_fun_times f g)"
+  proof
+    fix \<gamma>::"('a set)*('b set)"
+    assume pert: "\<gamma> \<in> (simplicial_complex_induced_by_monotone_boolean_function f) \<times> (simplicial_complex_induced_by_monotone_boolean_function g)"
+    hence "(fst \<gamma>) \<in> simplicial_complex_induced_by_monotone_boolean_function f"
+      by auto
+    hence sigma: "f (bool_vec_from_simplice (fst \<gamma>))"
+      by (metis (mono_tags, lifting) bool_vec_set_from_simplice_set_def boolean_function_from_simplicial_complex_def boolean_function_from_simplicial_complex_simplicial_complex_induced_by_monotone_boolean_function_id mem_Collect_eq)
+    from pert have "(snd \<gamma>) \<in> simplicial_complex_induced_by_monotone_boolean_function g"
+      by auto
+    hence tau: "g (bool_vec_from_simplice (snd \<gamma>))"
+      by (metis (mono_tags, lifting) bool_vec_set_from_simplice_set_def boolean_function_from_simplicial_complex_def boolean_function_from_simplicial_complex_simplicial_complex_induced_by_monotone_boolean_function_id mem_Collect_eq)
+    from sigma and tau have sigtau: "bool_fun_times f g (bool_vec_from_simplice ((fst \<gamma>) \<times> (snd \<gamma>)))"
+      using simp_ceros
+      unfolding bool_fun_times_def
+      unfolding set_fst_def
+      unfolding set_snd_def
+      by simp
+    from sigma and tau show "\<gamma> \<in> simplicial_complex_induced_by_monotone_boolean_function_times (bool_fun_times f g)"
+      using bool_vec_from_simplice_def ceros_of_boolean_input_in_set mem_Collect_eq simplicial_complex_induced_by_monotone_boolean_function_times_def
+      by blast
+  qed
+next
+  show "simplicial_complex_induced_by_monotone_boolean_function_ast (bool_fun_ast f g) \<subseteq> set_ast (simplicial_complex_induced_by_monotone_boolean_function f) (simplicial_complex_induced_by_monotone_boolean_function g)"
+  proof
+    fix \<gamma>::"'a set*'b set"
+    assume pert: "\<gamma> \<in> simplicial_complex_induced_by_monotone_boolean_function_ast (bool_fun_ast f g)"
+    hence sigma: "(fst \<gamma>) \<in> simplicial_complex_induced_by_monotone_boolean_function f"
+      by (smt (verit) bool_fun_ast_def fst_es_simplice mem_Collect_eq simplicial_complex_induced_by_monotone_boolean_function_def)
+    from pert have tau: "(snd \<gamma>) \<in> simplicial_complex_induced_by_monotone_boolean_function g"
+      by (smt (verit) bool_fun_ast_def snd_es_simplice mem_Collect_eq simplicial_complex_induced_by_monotone_boolean_function_def)
+    from sigma and tau show "\<gamma> \<in> set_ast (simplicial_complex_induced_by_monotone_boolean_function f) (simplicial_complex_induced_by_monotone_boolean_function g)"
+      using simp_ceros
+      by force
   qed
 qed
 
